fstar/new/Test.KeySchedule.fst
@@ -80,7 +80,7 @@ let gen_list_epoch_output cs group_id initial_init_secret l =
 
 val test_keyschedule_one: keyschedule_test -> ML bool
 let test_keyschedule_one t =
-  match uint16_to_ciphersuite t.cipher_suite with
+  match uint16_to_ciphersuite t.ks_cipher_suite with
   | Error s -> begin
     IO.print_string ("Skipping one test because of missing ciphersuite: '" ^ s ^ "'\n");
     true
