fstar/new/Test.TreeKEM.fst
@@ -1,0 +1,72 @@
+module Test.TreeKEM
+
+open FStar.IO
+open FStar.All
+open Test.Types
+open Test.Utils
+open Tree
+open TreeSync
+open TreeKEM
+open TreeSyncTreeKEMBinder
+open NetworkTypes
+open Parser
+open Lib.Result
+open Test.Utils
+open Lib.ByteSequence
+open Crypto
+
+val find_my_index: #l:nat -> #n:tree_size l -> treesync l n -> key_package_nt -> ML (res:nat{res<n})
+let find_my_index #l #n t kp =
+  let my_signature_key =
+    match kp.kpn_credential with
+    | C_basic c -> secret_to_pub c.bcn_signature_key
+    | _ -> failwith "unsupported credential!"; bytes_empty
+  in
+  let test (oc: option credential_t) =
+    match oc with
+    | None -> false
+    | Some c -> c.cred_signature_key = my_signature_key
+  in
+  let res = extract_option "couldn't find my_index" (find_first test (Seq.seq_to_list (tree_membership t))) in
+  res
+
+val test_treekem_one: treekem_test -> ML bool
+let test_treekem_one t =
+  if FStar.UInt16.v t.tk_cipher_suite <> 3 then (
+    IO.print_string "Skipping test because only Chacha20Poly1305 is supported\n";
+    true
+  ) else
+  match uint16_to_ciphersuite t.tk_cipher_suite with
+  | Error s -> begin
+    IO.print_string ("Skipping one test because of missing ciphersuite: '" ^ s ^ "'\n");
+    true
+  end
+  | Success cs -> begin
+    IO.print_string "Running test!!!\n";
+    let my_key_package = extract_option "bad key package" ((ps_to_pse ps_key_package).parse_exact (hex_string_to_bytes t.my_key_package)) in
+    let ratchet_tree = extract_option "bad ratchet tree" ((ps_to_pse ps_ratchet_tree).parse_exact (hex_string_to_bytes t.ratchet_tree_before)) in
+    let my_leaf_secret = (hex_string_to_bytes t.my_leaf_secret) in
+    let my_path_secret = (hex_string_to_bytes t.my_path_secret) in
+    let add_sender = FStar.UInt32.v t.add_sender in
+    let (|l, n|) = extract_result (ratchet_tree_l_n ratchet_tree) in
+    let ts0 = extract_result (ratchet_tree_to_treesync l n ratchet_tree) in
+    let tk0 = extract_result (treesync_to_treekem cs ts0) in
+    let my_index = find_my_index ts0 my_key_package in
+    if not (my_index <> add_sender) then
+      failwith ("new leaf cannot be equal to add_sender: my_index=" ^ nat_to_string my_index ^ " add_sender=" ^ nat_to_string add_sender ^ "\n")
+    else if not (add_sender < n) then
+      failwith "add_sender is too big"
+    else (
+      let upk0 = extract_result (mk_init_path tk0 my_index add_sender my_path_secret bytes_empty) in
+      let old_leaf_package = extract_result (key_package_to_treesync my_key_package) in
+      let ups0 = extract_result (treekem_to_treesync old_leaf_package upk0) in
+      let ts1 = apply_path dumb_credential ts0 ups0 in
+      let tk1 = extract_result (treesync_to_treekem cs ts1) in
+      let root_secret_after_add = extract_result (root_secret tk1 my_index my_leaf_secret bytes_empty) in
+      (bytes_to_hex_string root_secret_after_add) = t.root_secret_after_add
+    )
+  end
+
+val test_treekem: list treekem_test -> ML bool
+let test_treekem =
+  test_list "TreeKEM" test_treekem_one
