fstar/new/Test.fst
@@ -6,9 +6,10 @@ open Test.Types
 open Test.Reader
 open Test.TreeMath
 open Test.KeySchedule
+open Test.TreeKEM
 open Test.Utils
 
-let run_treemath_tests =
+let run_treemath_tests () =
   match get_testsuite TreeMath with
   | TreeMath_test l -> begin
     if test_treemath l then (
@@ -19,7 +20,7 @@ let run_treemath_tests =
   end
   | _ -> IO.print_string "TreeMath: got the wrong type of testsuite (internal error)\n"
 
-let run_keyschedule_tests =
+let run_keyschedule_tests () =
   match get_testsuite KeySchedule with
   | KeySchedule_test l -> begin
     if test_keyschedule l then (
@@ -30,6 +31,19 @@ let run_keyschedule_tests =
   end
   | _ -> IO.print_string "KeySchedule: got the wrong type of testsuite (internal error)\n"
 
+let run_treekem_tests () =
+  IO.print_string "Starting treekem\n";
+  match get_testsuite TreeKEM with
+  | TreeKEM_test l -> begin
+    if test_treekem l then (
+      IO.print_string ("TreeKEM: success (" ^ (nat_to_string (List.Tot.length l)) ^ " tests)\n")
+    ) else (
+      IO.print_string "TreeKEM: failure\n"
+    )
+  end
+  | _ -> IO.print_string "TreeKEM: got the wrong type of testsuite (internal error)\n"
+
 let main =
-  run_treemath_tests;
-  run_keyschedule_tests
+  run_treemath_tests ();
+  //run_keyschedule_tests ();
+  run_treekem_tests ()
